examples/raft/proof.v
@@ -1,0 +1,36 @@
+Require Import HoareDef SimModSem.
+Require Import Coqlib.
+Require Import ImpPrelude.
+Require Import Skeleton.
+Require Import PCM.
+Require Import ModSem Behavior.
+Require Import Relation_Definitions.
+Require Import src tgt header.
+Require Import HTactics ProofMode.
+
+
+Section SIMMODSEM.
+
+  Context `{Σ: GRA.t}.
+
+  Variable X: Type.
+
+  Let W: Type := Any.t * Any.t.
+
+  Let wf: _ -> W -> Prop :=
+    mk_wf (fun (_: unit) _ _ => (True: iProp)%I).
+
+  
+  Definition subset (A B: list X) := forall x, In x A -> In x B.
+
+
+  Theorem correct: refines2 [src.F] [tgt.F].
+Proof.
+  eapply adequacy_local2. econs; ss.
+    i. econstructor 1 with (wf:=wf) (le:=top2); et.
+    { ss. }
+- econs; ss. init. steps. unfold f. unfold src.f. steps. 
+    Admitted.
+
+End SIMMODSEM.
+
