examples/raft/skip.v
@@ -1,0 +1,275 @@
+Require Import Coqlib.
+Require Import ITreelib.
+Require Import ImpPrelude.
+Require Import STS.
+Require Import Behavior.
+Require Import ModSem.
+Require Import Skeleton.
+Require Import PCM.
+Require Import Imp.
+
+Require Import lmHeader.
+
+Set Implicit Arguments.
+
+Section H.
+  Definition popH: unit -> itree Es unit :=
+    fun varg =>
+    Ret tt
+  .
+
+  Definition pushH: unit -> itree Es unit :=
+    fun varg =>
+    Ret tt
+  .
+
+  Definition HSem: ModSem.t := {|
+    ModSem.fnsems := [("popH", cfunU popH); ("pushH", cfunU pushH)];
+    ModSem.mn := "H";
+    ModSem.initial_st := (@nil val)↑; (* queue or list *)
+  |}
+  .
+  Definition H: Mod.t := {|
+    Mod.get_modsem := fun _ => HSem;
+    Mod.sk := [("popH", Gfun↑); ("pushH", Gfun↑)];
+  |}
+  .
+
+End H.
+
+
+Section CC.
+  (* Queue *)
+
+  Definition pop: list val -> itree Es val := 
+    fun varg =>
+    st <- trigger PGet;;
+    `l : (list val) <- st↓?;;
+    let '(x, l) := match l with | h::t => (h, t) | _ => ((Vint 0), (@nil val)) end in
+    trigger (PPut l↑);;; 
+    Ret x
+  .
+  Definition push: list val -> itree Es val := 
+    fun varg =>
+    `x: val <- (pargs [Tuntyped] varg)?;;
+    st <- trigger PGet;;
+    `l : (list val) <- st↓?;;
+    let l := l ++ [x] in
+    trigger (PPut l↑);;;
+    Ret Vundef
+  .
+
+  (* Debug *)
+  Definition print: unit -> itree Es unit :=
+    fun varg =>
+      st <- trigger PGet;;
+      `l : (list val) <- st↓?;;
+      _ <- (ITree.iter
+        (fun i =>
+          _ <- (match i with
+          | h::t => (printV h)
+          | _ => (printV (Vint 0)) 
+          end);;
+          match i with
+          | h::t => Ret (inl t)
+          | _ => Ret (inr tt)
+          end
+        ) l);;
+
+      Ret tt
+    .
+
+
+
+  Definition CCSem: ModSem.t := {|
+    ModSem.fnsems := [("pop", cfunU pop); ("push", cfunU push); ("print", cfunU print)];
+    ModSem.mn := "CC";
+    ModSem.initial_st := (@nil val)↑; (* queue or list *)
+  |}
+  .
+  Definition CC: Mod.t := {|
+    Mod.get_modsem := fun _ => CCSem;
+    Mod.sk := [("pop", Gfun↑); ("push", Gfun↑); ("print", Gfun↑)];
+  |}
+  .
+
+End CC.
+
+Section F.
+  (* Simple function using push, pop + @ *)
+  (* getint x ; yield ; push 2*x ; yield *)
+  Definition f: list val -> itree Es val :=
+  fun varg =>
+    `x: val <- (pargs [Tuntyped] varg)?;;
+    _ <- trigger EventsL.Yield;;
+    x <- (vadd x (Vint 1))?;;
+    trigger (Call "push" [x]↑);;;
+    trigger (Call "pushH" []);;;
+    _ <- trigger EventsL.Yield;;
+    Ret Vundef
+  .
+
+  Definition FSem: ModSem.t := {|
+    ModSem.fnsems := [("f", cfunU f)];
+    ModSem.mn := "F";
+    ModSem.initial_st := tt↑;
+  |}
+  .
+
+  Definition F: Mod.t := {|
+    Mod.get_modsem := fun _ => FSem;
+    Mod.sk := [("f", Gfun↑)];
+  |}
+  .
+
+End F.
+
+Section G.
+  (* Simple function using push, pop + @*)
+  (* yield; x = pop; yield; return x/2 *)
+  Definition g: list val -> itree Es val :=
+  fun varg =>
+    _ <- trigger EventsL.Yield;;
+    `x : val <- ccallU "pop" (@nil val);;
+    `x : val <- ccallU "popH" (@nil val);;
+    _ <- trigger EventsL.Yield;;
+    x <- (vsub x (Vint 1))?;;
+    Ret x
+  .
+
+
+  Definition GSem: ModSem.t := {|
+    ModSem.fnsems := [("g", cfunU g)];
+    ModSem.mn := "G";
+    ModSem.initial_st := tt↑;
+  |}
+  .
+
+  Definition G: Mod.t := {|
+    Mod.get_modsem := fun _ => GSem;
+    Mod.sk := [("g", Gfun↑)];
+  |}
+  .
+
+End G.
+
+Section MAIN.
+  Definition main : option mname * Any.t-> itree Es Any.t :=
+  fun '(_, varg) =>
+  trigger (EventsL.Spawn "threadF" (@nil val)↑);;; 
+  trigger (EventsL.Spawn "threadF" (@nil val)↑);;; 
+  trigger (EventsL.Spawn "threadF" (@nil val)↑);;; 
+  trigger (EventsL.Spawn "threadG" (@nil val)↑);;; 
+  trigger (EventsL.Spawn "threadG" (@nil val)↑);;; 
+  trigger (EventsL.Spawn "threadG" (@nil val)↑);;; 
+  trigger (EventsL.Spawn "threadP" (@nil val)↑);;; 
+
+  Ret Vundef↑
+  .
+  
+  Definition MainSem: ModSem.t := {|
+    ModSem.fnsems := [("main", main)];
+    ModSem.mn := "Main";
+    ModSem.initial_st := tt↑;
+  |}
+  .
+  
+  Definition Main: Mod.t := {|
+    Mod.get_modsem := fun _ => MainSem;
+    Mod.sk := Sk.unit;
+  |}
+  .
+
+End MAIN.
+
+
+Section TH1.
+  Definition threadF : option mname * Any.t-> itree Es Any.t :=
+  fun '(_, varg) =>
+    let i := (Vint 0) in
+    `_:unit <- (ITree.iter
+    ( fun i =>
+    `_:val <- ccallU "f" [i];;
+    i' <- (vadd i (Vint 1))?;;
+    Ret (inl i')
+    ) i );;
+
+   
+   Ret Vundef↑
+  .
+
+  Definition TH1Sem: ModSem.t := {|
+    ModSem.fnsems := [("threadF", threadF)];
+    ModSem.mn := "TH1";
+    ModSem.initial_st := tt↑;
+
+  |}
+  .
+
+  Definition TH1: Mod.t := {|
+    Mod.get_modsem := fun _ => TH1Sem;
+    Mod.sk := Sk.unit;
+  |}
+  .
+
+End TH1.
+
+Section TH2.
+  Definition threadG : option mname * Any.t-> itree Es Any.t :=
+    fun '(_, varg) =>
+      `_:unit <- (ITree.iter
+        ( fun _ =>
+        `_:val <- ccallU "g" (@nil val);;
+        Ret (inl tt)
+        ) tt );;
+
+   
+   Ret Vundef↑
+  .
+
+  Definition TH2Sem: ModSem.t := {|
+    ModSem.fnsems := [("threadG", threadG)];
+    ModSem.mn := "TH2";
+    ModSem.initial_st := tt↑;
+
+  |}
+  .
+
+  Definition TH2: Mod.t := {|
+    Mod.get_modsem := fun _ => TH2Sem;
+    Mod.sk := Sk.unit;
+  |}
+  .
+
+
+End TH2.
+Section TH3. 
+(* Print *)
+
+  Definition threadP : option mname * Any.t -> itree Es Any.t :=
+  fun '(_, varg) =>
+  `_:unit <- (ITree.iter
+        ( fun _ =>
+        `_:val <- ccallU "print" tt;;
+        _ <- trigger EventsL.Yield;;
+        Ret (inl tt)
+        ) tt
+  );;
+
+  Ret Vundef↑
+.
+  Definition TH3Sem: ModSem.t := {|
+    ModSem.fnsems := [("threadP", threadP)];
+    ModSem.mn := "TH3";
+    ModSem.initial_st := tt↑;
+
+  |}
+  .
+
+  Definition TH3: Mod.t := {|
+    Mod.get_modsem := fun _ => TH3Sem;
+    Mod.sk := Sk.unit;
+  |}
+  .
+
+End TH3.
