examples/raft/src.v
@@ -1,0 +1,150 @@
+Require Import Coqlib.
+Require Import ITreelib.
+Require Import ImpPrelude.
+Require Import STS.
+Require Import Behavior.
+Require Import ModSem.
+Require Import Skeleton.
+Require Import Imp.
+
+
+
+
+Section H.
+  (* Queue *)
+
+  Definition popH: list val -> itree Es val := 
+    fun varg =>
+    st <- trigger sGet;;
+    `l : (list val) <- st↓?;;
+    let '(x, l) := match l with | h::t => (h, t) | _ => ((Vint 0), (@nil val)) end in
+    x <- (vsub x (Vint 1))?;;
+    trigger (sPut l↑);;; 
+    Ret x
+  .
+  Definition pushH: list val -> itree Es val := 
+    fun varg =>
+    `x: val <- (pargs [Tuntyped] varg)?;;
+    st <- trigger sGet;;
+    `l : (list val) <- st↓?;;
+    x <- (vadd x (Vint 1))?;;
+    let l := l ++ [x] in
+    trigger (sPut l↑);;;
+    Ret Vundef
+  .
+  Definition HSem: ModSem.t := {|
+    ModSem.fnsems := [("popH", cfunU popH); ("pushH", cfunU pushH)];
+    ModSem.init_st := (@nil val)↑; (* queue or list *)
+  |}
+  .
+  Definition H: Mod.t := {|
+    Mod.get_modsem := fun _ => HSem;
+    Mod.sk := [("popH", Gfun↑); ("pushH", Gfun↑)];
+  |}
+  .
+
+End H.
+
+Section CC.
+  Definition pop: unit -> itree Es unit :=
+  fun varg =>
+    Ret tt
+  .
+
+  Definition push: unit -> itree Es unit :=
+  fun varg =>
+    Ret tt
+  .
+
+  Definition CCSem: ModSem.t := {|
+    ModSem.fnsems := [("pop", cfunU pop); ("push", cfunU push)];
+    ModSem.mn := "CC";
+    ModSem.initial_st := tt↑; (* queue or list *)
+  |}
+  .
+  Definition CC: Mod.t := {|
+    Mod.get_modsem := fun _ => CCSem;
+    Mod.sk := [("pop", Gfun↑); ("push", Gfun↑)];
+  |}
+  .
+
+
+End CC.
+
+Section F.
+  (* Simple function using push, pop + @ *)
+  (* getint x ; yield ; push x ; yield *)
+  Definition f: list val -> itree Es val :=
+  fun varg =>
+    `x: val <- (pargs [Tuntyped] varg)?;;
+    _ <- trigger EventsL.Yield;;
+    trigger (Call "pushH" [x]↑);;;
+    _ <- trigger EventsL.Yield;;
+    Ret Vundef
+  .
+
+  Definition FSem: ModSem.t := {|
+    ModSem.fnsems := [("f", cfunU f)];
+    ModSem.mn := "F";
+    ModSem.initial_st := tt↑;
+  |}
+  .
+
+  Definition F: Mod.t := {|
+    Mod.get_modsem := fun _ => FSem;
+    Mod.sk := [("f", Gfun↑)];
+  |}
+  .
+
+End F.
+
+Section G.
+  (* Simple function using push, pop + @*)
+  (* yield; x = pop; yield; return x *)
+  Definition g: list val -> itree Es val :=
+  fun varg =>
+    _ <- trigger EventsL.Yield;;
+    `x : val <- ccallU "popH" (@nil val);;
+    _ <- trigger EventsL.Yield;;
+    Ret x
+  .
+
+
+  Definition GSem: ModSem.t := {|
+    ModSem.fnsems := [("g", cfunU g)];
+    ModSem.mn := "G";
+    ModSem.initial_st := tt↑;
+  |}
+  .
+
+  Definition G: Mod.t := {|
+    Mod.get_modsem := fun _ => GSem;
+    Mod.sk := [("g", Gfun↑)];
+  |}
+  .
+
+End G.
+
+
+
+Section MAIN.
+  Definition main : option mname * Any.t-> itree Es Any.t :=
+  fun '(_, varg) =>
+  trigger (Call "pushH" [(Vint 10)]↑);;;
+  Ret Vundef↑
+  .
+  
+  Definition MainSem: ModSem.t := {|
+    ModSem.fnsems := [("main", main)];
+    ModSem.mn := "Main";
+    ModSem.initial_st := tt↑;
+  |}
+  .
+  
+  Definition Main: Mod.t := {|
+    Mod.get_modsem := fun _ => MainSem;
+    Mod.sk := Sk.unit;
+  |}
+  .
+
+End MAIN.
