examples/raft/src_main.v
@@ -1,0 +1,17 @@
+Require Import Coqlib.
+Require Import ITreelib.
+Require Import Skeleton.
+Require Import PCM.
+Require Import STS Behavior.
+Require Import Any.
+Require Import ModSem.
+Require Import ImpPrelude.
+
+Require Import src.
+
+Set Implicit Arguments.
+
+Definition srcModules : list Mod.t := [src.H; src.CC; src.F; src.G; src.Main].
+
+Definition test_itr := ModSemL.initial_itr (ModL.enclose (Mod.add_list srcModules)) None.
+
