examples/raft/tgt_main.v
@@ -1,0 +1,17 @@
+Require Import Coqlib.
+Require Import ITreelib.
+Require Import Skeleton.
+Require Import PCM.
+Require Import STS Behavior.
+Require Import Any.
+Require Import ModSem.
+Require Import ImpPrelude.
+
+Require Import tgt.
+
+Set Implicit Arguments.
+
+Definition tgtModules : list Mod.t := [tgt.H; tgt.CC; tgt.F; tgt.G; tgt.Main; TH1; TH2; TH3].
+
+Definition test_itr := ModSemL.initial_itr (ModL.enclose (Mod.add_list tgtModules)) None.
+
